update

unionfind.dfy
@@ -11,20 +11,26 @@
         ensures forall i :: 0 <= i < n ==> 
             MultimiDisjuncte(seq(n, i => i), seq(n, i => 0)).parinte[i] == i &&
             MultimiDisjuncte(seq(n, i => i), seq(n, i => 0)).rang[i] == 0
+        ensures validMultimi(Initial(n))
     {
         MultimiDisjuncte(
             parinte := seq(n, i => i), 
             rang := seq(n, i => 0)
         )
     }
-// predicate validMultimi()
+predicate validMultimi(md: MultimiDisjuncte){
+    |md.parinte| == |md.rang| && forall x  :: 0 <= x < |md.parinte| ==> 0 <= md.parinte[x] < |md.parinte|
+}
 
 // Method to find the leader of a set (with path compression)
     method Cautare(md: MultimiDisjuncte, x: int) returns (lider: int, updated: MultimiDisjuncte)
         requires 0 <= x < |md.parinte|
+        requires validMultimi(md)
         ensures 0 <= lider < |md.parinte|
         ensures 0 <= lider < |updated.parinte|
         ensures updated.parinte[lider] == lider
+        ensures validMultimi(updated)
+        ensures |md.parinte| == |updated.parinte|
         decreases *
         //ensures forall i :: 0 <= i < |md.parinte| && old(md.parinte[i]) == i ==> updated.parinte[i] == lider
     {
@@ -45,11 +51,14 @@
 method Unire(md: MultimiDisjuncte, x: int, y: int) returns (updated: MultimiDisjuncte)
     requires 0 <= x < |md.parinte|
     requires 0 <= y < |md.parinte|
-    ensures 0 <= x < |updated.parinte|
-    ensures 0 <= y < |updated.parinte|
-    ensures updated.parinte[x] == updated.parinte[y] 
-    ensures forall i :: 0 <= i < |md.parinte| ==> 
-        (exists lider :: 0 <= lider < |md.parinte| && updated.parinte[i] == lider)
+    requires validMultimi(md)
+    // modifies md // metoda modifica md
+    ensures validMultimi(updated)  
+    requires 0 <= x < |md.parinte|
+    requires 0 <= y < |md.parinte|
+    // ensures updated.parinte[x] == updated.parinte[y] 
+    // ensures forall i :: 0 <= i < |md.parinte| ==> 
+    //     (exists lider :: 0 <= lider < |md.parinte| && updated.parinte[i] == lider)
     decreases *
 {
     var liderX, state1 := Cautare(md, x);
@@ -57,17 +66,13 @@ method Unire(md: MultimiDisjuncte, x: int, y: int) returns (updated: MultimiDisj
 
     if liderX != liderY {
         if state2.rang[liderX] < state2.rang[liderY] {
-            state2.parinte := state2.parinte[liderX := liderY];
-            updated := state2;
+            updated:= MultimiDisjuncte(state2.parinte[liderX := liderY], state2.rang);
         } else if state2.rang[liderX] > state2.rang[liderY] {
-            state2.parinte := state2.parinte[liderY := liderX];
-            updated := state2;
+            updated:= MultimiDisjuncte(state2.parinte[liderY := liderX], state2.rang); 
         } else {
-            state2.parinte := state2.parinte[liderY := liderX];
-            state2.rang := state2.rang[liderX := state2.rang[liderX] + 1];
-            updated := state2;
+            updated:= MultimiDisjuncte(state2.parinte[liderY := liderX], state2.rang);
+            updated:= MultimiDisjuncte(state2.rang[liderX := liderX], state2.parinte);
         }
-    } else {
-        updated := state2;
     }
+    updated := state2;
 }
